theories/serialization/Serialize.v
@@ -7,14 +7,24 @@ From Peregrine Require CeresExtra.
 
 
 
-Definition program_of_string := SerializeEAst.program_of_string.
-
-Definition global_env_of_string := SerializeExAst.global_env_of_string.
-
-Definition kername_of_string := SerializeCommon.kername_of_string.
-
 Definition string_of_error := CeresExtra.string_of_error.
 
 Definition PAst_of_string := SerializePAst.PAst_of_string.
 
 Definition config_of_string := SerializeConfig.config'_of_string.
+
+Definition backend_config_of_string := SerializeConfig.backend_config'_of_string.
+
+Definition erasure_phases_of_string := SerializeConfig.erasure_phases'_of_string.
+
+Definition attributes_config_of_string := SerializeConfig.attributes_config_of_string.
+
+
+(* TODO: remove? *)
+Definition program_of_string := SerializeEAst.program_of_string.
+
+(* TODO: remove? *)
+Definition global_env_of_string := SerializeExAst.global_env_of_string.
+
+(* TODO: remove? *)
+Definition kername_of_string := SerializeCommon.kername_of_string.
