theories/serialization/SerializeConfigSound.v
@@ -433,3 +433,21 @@ Proof.
   rewrite <- Ea0, <- Ea1, <- Ea2, <- Ea3, <- Ea4, <- Ea5.
   reflexivity.
 Qed.
+
+Instance Sound_attributes_config : SoundClass attributes_config.
+Proof.
+  unfold SoundClass, Sound.
+  intros l e a He.
+  apply sound_match_con in He.
+  destruct He as [He | He]; elim_Exists He.
+  destruct He as [es [<- He]].
+  sound_field He.
+  apply sound_class in Ea0.
+  apply sound_class in Ea1.
+  apply sound_class in Ea2.
+  apply sound_class in Ea3.
+  unfold to_sexp, Serialize_attributes_config.
+  cbn.
+  rewrite <- Ea0, <- Ea1, <- Ea2, <- Ea3.
+  reflexivity.
+Qed.
